Refactor namespaces and corruption definition.

nsl.v
@@ -25,59 +25,73 @@ Class nslG := {
 
 Context `{!nslG}.
 
+Definition corruption kA kB : iProp :=
+  pterm (TKey Dec kA) ∨ pterm (TKey Dec kB).
+
 Definition msg1_pred (kB : term) m1 : iProp :=
   ∃ nA kA, ⌜m1 = Spec.of_list [nA; TKey Enc kA]⌝ ∧
-           (pterm nA ↔ ▷ (pterm (TKey Dec kA) ∨ pterm (TKey Dec kB))) ∧
+           (pterm nA ↔ ▷ corruption kA kB) ∧
            pterm (TKey Enc kA).
 
 Definition msg2_pred kA m2 : iProp :=
   ∃ nA nB kB,
     ⌜m2 = Spec.of_list [nA; nB; TKey Enc kB]⌝ ∧
-    (pterm nB ↔ ▷ (pterm (TKey Dec kA) ∨ pterm (TKey Dec kB))) ∧
+    (pterm nB ↔ ▷ corruption kA kB) ∧
     session nsl_sess_name Resp kA kB nA nB.
 
 Definition msg3_pred kB nB : iProp :=
   ∀ nA kA,
     session nsl_sess_name Resp kA kB nA nB -∗
     session nsl_sess_name Init kA kB nA nB ∧
-    (pterm nA ↔ ▷ (pterm (TKey Dec kA) ∨ pterm (TKey Dec kB))).
+    (pterm nA ↔ ▷ corruption kA kB).
+
+Variable N : namespace.
 
 Variable nsl_sess_inv : role → term → term → term → term → iProp.
 
 Definition nsl_inv : iProp :=
-  session_inv nsl_sess_name (cryptoN.@"nsl") nsl_sess_inv.
+  session_inv nsl_sess_name N nsl_sess_inv.
 
 Definition nsl_ctx : iProp :=
-  session_ctx nsl_sess_name (cryptoN.@"nsl") nsl_sess_inv.
+  session_ctx nsl_sess_name N nsl_sess_inv ∧
+  crypto_enc (N.@"m1") msg1_pred ∧
+  crypto_enc (N.@"m2") msg2_pred ∧
+  crypto_enc (N.@"m3") msg3_pred.
+
+Global Instance persistent_nsl_ctx : Persistent nsl_ctx.
+Proof. apply _. Qed.
+
+Lemma nsl_ctx_session_ctx :
+  nsl_ctx -∗
+  session_ctx nsl_sess_name N nsl_sess_inv.
+Proof. by iIntros "( ? & ? )". Qed.
 
 Variable send recv : val.
 
 Ltac protocol_failure :=
   by intros; wp_pures; iApply ("Hpost" $! None).
 
-Definition initiator : val := λ: "skA" "pkA" "pkB" "nA",
-  bind: "m1"   := tenc (nroot.@"m1") "pkB" (term_of_list ["nA"; "pkA"]) in
+Definition nsl_init : val := λ: "skA" "pkA" "pkB" "nA",
+  bind: "m1"   := tenc (N.@"m1") "pkB" (term_of_list ["nA"; "pkA"]) in
   send "m1";;
-  bind: "m2"   := tdec (nroot.@"m2") "skA" (recv #()) in
+  bind: "m2"   := tdec (N.@"m2") "skA" (recv #()) in
   bind: "m2"   := list_of_term "m2" in
   list_match: ["nA'"; "nB"; "pkB'"] := "m2" in
-  if: eq_term "nA'" "nA" && eq_term "pkB'" "pkB" then
-    bind: "m3" := tenc (nroot.@"m3") "pkB" "nB" in
-    send "m3";;
-    SOME "nB"
-  else NONE.
+  assert: eq_term "nA'" "nA" && eq_term "pkB'" "pkB" in
+  bind: "m3" := tenc (N.@"m3") "pkB" "nB" in
+  send "m3";;
+  SOME "nB".
 
-Definition responder : val := λ: "skB" "pkB" "nB",
-  bind: "m1" := tdec (nroot.@"m1") "skB" (recv #()) in
+Definition nsl_resp : val := λ: "skB" "pkB" "nB",
+  bind: "m1" := tdec (N.@"m1") "skB" (recv #()) in
   bind: "m1" := list_of_term "m1" in
   list_match: ["nA"; "pkA"] := "m1" in
   bind: "kt" := is_key "pkA" in
-  if: "kt" = repr Enc then
-    bind: "m2" := tenc (nroot.@"m2") "pkA" (term_of_list ["nA"; "nB"; "pkB"]) in
-    send "m2";;
-    bind: "m3" := tdec (nroot.@"m3") "skB" (recv #()) in
-    if: eq_term "m3" "nB" then SOME ("pkA", "nA") else NONE
-  else NONE.
+  assert: "kt" = repr Enc in
+  bind: "m2" := tenc (N.@"m2") "pkA" (term_of_list ["nA"; "nB"; "pkB"]) in
+  send "m2";;
+  bind: "m3" := tdec (N.@"m3") "skB" (recv #()) in
+  assert: eq_term "m3" "nB" in SOME ("pkA", "nA").
 
 Implicit Types Ψ : val → iProp.
 
@@ -91,14 +105,14 @@ Hypothesis wp_recv : forall E Ψ,
   WP recv #() @ E {{ Ψ }}.
 
 Lemma pterm_msg1I kA kB (nA : term) :
-  crypto_enc (nroot.@"m1") msg1_pred -∗
+  nsl_ctx -∗
   pterm (TKey Enc kA) -∗
   sterm nA -∗
-  □ (pterm nA ↔ ▷ (pterm (TKey Dec kA) ∨ pterm (TKey Dec kB))) -∗
+  □ (pterm nA ↔ ▷ corruption kA kB) -∗
   pterm (TKey Enc kB) -∗
-  ▷ pterm (TEnc kB (Spec.tag (nroot.@"m1") (Spec.of_list [nA; TKey Enc kA]))).
+  ▷ pterm (TEnc kB (Spec.tag (N.@"m1") (Spec.of_list [nA; TKey Enc kA]))).
 Proof.
-iIntros "#Hm1 #HkA #HnA #HnA_hi #HkB".
+iIntros "(_ & #Hm1 & _ & _) #HkA #HnA #HnA_hi #HkB".
 iModIntro.
 iApply pterm_TEncIS; eauto.
 - by iApply pterm_sterm.
@@ -108,21 +122,21 @@ iApply pterm_TEncIS; eauto.
   by iApply pterm_sterm.
 - iIntros "!> HkB_dec".
   rewrite pterm_of_list /=; do !iSplit => //.
-  iApply "HnA_hi"; eauto.
+  by iApply "HnA_hi"; rewrite /corruption; eauto.
 Qed.
 
 Lemma pterm_msg2I kA kB nA nB :
-  crypto_enc (nroot.@"m2") msg2_pred -∗
+  nsl_ctx -∗
   ▷ pterm (TKey Enc kA) -∗
   pterm (TKey Enc kB) -∗
   sterm nA -∗
   □ (pterm (TKey Dec kA) → pterm nA) -∗
   sterm nB -∗
-  □ (pterm nB ↔ ▷ (pterm (TKey Dec kA) ∨ pterm (TKey Dec kB))) -∗
+  □ (pterm nB ↔ ▷ corruption kA kB) -∗
   session nsl_sess_name Resp kA kB nA nB -∗
-  ▷ pterm (TEnc kA (Spec.tag (nroot.@"m2") (Spec.of_list [nA; nB; TKey Enc kB]))).
+  ▷ pterm (TEnc kA (Spec.tag (N.@"m2") (Spec.of_list [nA; nB; TKey Enc kB]))).
 Proof.
-iIntros "#Hm2 #HAenc #HBenc #HnAhi #HnAlo #HnBhi #HnBlo #sess !>".
+iIntros "# (_ & _ & Hm2 & _) #HAenc #HBenc #HnAhi #HnAlo #HnBhi #HnBlo #sess !>".
 iApply pterm_TEncIS; eauto.
 - by iApply pterm_sterm.
 - iModIntro; iExists _, _, _; do !iSplit => //.
@@ -131,17 +145,16 @@ iApply pterm_TEncIS; eauto.
 iIntros "!> #pub".
 iSpecialize ("HnAlo" with "pub").
 rewrite pterm_of_list /=; do !iSplit => //.
-by iApply "HnBlo"; eauto.
+by iApply "HnBlo"; rewrite /corruption; eauto.
 Qed.
 
 Lemma pterm_msg1E kA kB nA :
-  crypto_enc (nroot.@"m1") msg1_pred -∗
-  pterm (TEnc kB (Spec.tag (nroot.@"m1") (Spec.of_list [nA; TKey Enc kA]))) -∗
+  nsl_ctx -∗
+  pterm (TEnc kB (Spec.tag (N.@"m1") (Spec.of_list [nA; TKey Enc kA]))) -∗
   ▷ (pterm (TKey Enc kA) ∧ sterm nA ∧
-     (pterm nA ∨
-      □ (pterm nA ↔ ▷ (pterm (TKey Dec kA) ∨ pterm (TKey Dec kB))))).
+     (pterm nA ∨ (pterm nA ↔ ▷ corruption kA kB))).
 Proof.
-iIntros "#m1P #Hts".
+iIntros "# (_ & m1P & _ & _) #Hts".
 iDestruct (pterm_TEncE with "Hts [//]") as "{Hts} [[HkB Hts]|Hts]".
   rewrite pterm_of_list /=.
   iDestruct "Hts" as "(HnA & HkA & _)".
@@ -155,37 +168,73 @@ by eauto.
 Qed.
 
 Lemma pterm_msg2E kA kB nA nB :
-  crypto_enc (nroot.@"m2") msg2_pred -∗
-  pterm (TEnc kA (Spec.tag (nroot.@"m2") (Spec.of_list [nA; nB; TKey Enc kB]))) -∗
+  nsl_ctx -∗
+  □ (pterm nA ↔ ▷ corruption kA kB) -∗
+  pterm (TEnc kA (Spec.tag (N.@"m2") (Spec.of_list [nA; nB; TKey Enc kB]))) -∗
   ▷ (sterm nB ∧
-     (pterm nA ∧ pterm nB ∨
-      □ (pterm nB ↔ ▷ (pterm (TKey Dec kA) ∨ pterm (TKey Dec kB))) ∧
-      session nsl_sess_name Resp kA kB nA nB)).
+     (pterm nB ↔ ▷ corruption kA kB) ∧
+     ▷ (corruption kA kB ∨
+        session nsl_sess_name Resp kA kB nA nB)).
 Proof.
-iIntros "#? #Hts".
-iDestruct (pterm_TEncE with "Hts [//]") as "{Hts} [[_ Hts] | Hts]".
+iIntros "# (_ & _ & ? & _) #p_nA #Hts".
+iDestruct (pterm_TEncE with "Hts [//]") as "{Hts} [[? Hts] | Hts]".
   rewrite pterm_of_list /=.
-  iDestruct "Hts" as "(? & ? & ? & ?)".
+  iDestruct "Hts" as "(p_nA' & ? & ? & ?)".
   iAssert (sterm nB) as "#?". by iApply pterm_sterm.
-  by eauto.
+  iPoseProof ("p_nA" with "p_nA'") as "?".
+  by do 3![iSplit; eauto].
 iDestruct "Hts" as "(#inv & Hts & _)"; iModIntro.
 iDestruct "inv" as (nA' nB' kB') "(%e_m & #nBP & frag)".
 case/Spec.of_list_inj: e_m => <- <- <-; rewrite sterm_of_list /=.
 iDestruct "Hts" as "(?&?&?)"; by eauto.
 Qed.
 
-Lemma wp_initiator kA kB (nA : term) E Ψ :
-  ↑cryptoN.@"nsl" ⊆ E →
+Lemma pterm_msg3I kA kB nA nB :
   nsl_ctx -∗
-  crypto_enc (nroot.@"m1") msg1_pred -∗
-  crypto_enc (nroot.@"m2") msg2_pred -∗
-  crypto_enc (nroot.@"m3") msg3_pred -∗
+  pterm (TKey Enc kA) -∗
+  pterm (TKey Enc kB) -∗
+  □ (pterm nA ↔ ▷ corruption kA kB) -∗
+  sterm nB -∗
+  □ (pterm nB ↔ ▷ corruption kA kB) -∗
+  session nsl_sess_name Resp kA kB nA nB -∗
+  session nsl_sess_name Init kA kB nA nB -∗
+  pterm (TEnc kB (Spec.tag (N.@"m3") nB)).
+Proof.
+iIntros "(_ & _ & _ & #Hm3) #p_kA #p_kB #p_nA #s_nB #p_nB #sessA #sessB".
+iApply pterm_TEncIS => //.
+- by iApply pterm_sterm.
+- iModIntro. iIntros (nA' kA') "#sessA'".
+  iDestruct (session_agree with "sessA sessA'") as "(-> & _ & -> & _)" => //.
+  by iSplit.
+by iIntros "!> ?"; iApply "p_nB"; rewrite /corruption; eauto.
+Qed.
+
+Lemma pterm_msg3E kA kB nA nB :
+  nsl_ctx -∗
+  session nsl_sess_name Resp kA kB nA nB -∗
+  □ (pterm nB ↔ ▷ corruption kA kB) -∗
+  pterm (TEnc kB (Spec.tag (N.@"m3") nB)) -∗
+  ▷ (corruption kA kB ∨
+     session nsl_sess_name Init kA kB nA nB ∧
+     (pterm nA ↔ ▷ corruption kA kB)).
+Proof.
+iIntros "(_ & _ & _ & #Hm3) #sessB #p_nB #p_m3".
+iDestruct (pterm_TEncE with "p_m3 [//]") as "[[_ fail]|inv]".
+  by iLeft; iApply "p_nB".
+iDestruct "inv" as "(#inv & _ & _)".
+iModIntro; iRight.
+by iApply "inv".
+Qed.
+
+Lemma wp_nsl_init kA kB (nA : term) E Ψ :
+  ↑N ⊆ E →
+  nsl_ctx -∗
   pterm (TKey Enc kA) -∗
   pterm (TKey Enc kB) -∗
   sterm nA -∗
   □ (pterm nA ↔ ▷ (pterm (TKey Dec kA) ∨ pterm (TKey Dec kB))) -∗
-  (∀ nB, pterm nA ∨ nsl_sess_inv Init kA kB nA nB) -∗
-  crypto_meta_token nA (↑cryptoN.@"nsl".@nA) -∗
+  (∀ nB, nsl_sess_inv Init kA kB nA nB) -∗
+  crypto_meta_token nA (↑N) -∗
   (∀ onB : option term,
       (if onB is Some nB then
          sterm nB ∧
@@ -193,11 +242,11 @@ Lemma wp_initiator kA kB (nA : term) E Ψ :
            nsl_sess_inv Resp kA kB nA nB)
        else True) -∗
       Ψ (repr onB)) -∗
-  WP initiator (TKey Dec kA) (TKey Enc kA) (TKey Enc kB) nA @ E
+  WP nsl_init (TKey Dec kA) (TKey Enc kA) (TKey Enc kB) nA @ E
      {{ Ψ }}.
 Proof.
-rewrite /initiator.
-iIntros (?) "#ctx #? #? #? #enc_kA #enc_kB #s_nA #p_nA inv unreg Hpost".
+rewrite /nsl_init.
+iIntros (?) "#ctx #enc_kA #enc_kB #s_nA #p_nA inv unreg Hpost".
 wp_list (_ :: _ :: []).
 wp_term_of_list.
 wp_tenc => /=.
@@ -214,41 +263,29 @@ case: m2 => [|??] /=; wp_pures; last protocol_failure.
 wp_eq_term e; last protocol_failure; subst nA'.
 wp_eq_term e; last protocol_failure; subst pkB'.
 wp_tenc.
-iPoseProof (pterm_msg2E with "[//] Hm2") as "{Hm2} [HnB Hm2]"; eauto.
-wp_pures; iDestruct "Hm2" as "[[p_nA' ?]|[p_nB sessB]]".
-  iSpecialize ("p_nA" with "p_nA'").
+iPoseProof (pterm_msg2E with "[//] [//] Hm2")
+  as "{Hm2} (s_nB & p_nB & Hm2)"; eauto.
+wp_pures; iDestruct "Hm2" as "[fail|sessB]".
   wp_bind (send _); iApply wp_send.
     iModIntro; iApply pterm_TEncIP => //.
-    by rewrite pterm_tag.
+    by rewrite pterm_tag; iApply "p_nB".
   by wp_pures; iApply ("Hpost" $! (Some nB)); eauto.
-iDestruct ("inv" $! nB) as "[#p_nA' | inv]".
-  iSpecialize ("p_nA" with "p_nA'").
-  wp_bind (send _); iApply wp_send.
-    iModIntro; iApply pterm_TEncIP => //.
-    by rewrite pterm_tag; iApply "p_nB"; iApply "p_nA".
-  by wp_pures; iApply ("Hpost" $! (Some nB)); eauto.
+iSpecialize ("inv" $! nB).
 iMod (session_begin with "[] inv [unreg]") as "[#sessA close]" => //.
+  by iApply nsl_ctx_session_ctx.
 iMod ("close" with "sessB") as "inv_resp" => //=.
 wp_bind (send _); iApply wp_send.
-  iModIntro; iApply pterm_TEncIS; eauto.
-  - by iApply pterm_sterm.
-  - iIntros "!> %nA' %kA' #sessB'".
-    iDestruct (session_agree with "sessB' sessB") as "/= %e" => //.
-    by case: e => [] -> [] _ [] -> _; iSplit => //.
-  - iIntros "!> #dec_kB". iApply "p_nB". by eauto.
+  by iModIntro; iApply (pterm_msg3I with "[] [] [] [] [] [] sessB sessA"); eauto.
 wp_pures; iApply ("Hpost" $! (Some nB)); eauto.
 Qed.
 
-Lemma wp_responder kB E Ψ nB :
-  ↑cryptoN.@"nsl" ⊆ E →
+Lemma wp_nsl_resp kB E Ψ nB :
+  ↑N ⊆ E →
   nsl_ctx -∗
-  crypto_enc (nroot.@"m1") msg1_pred -∗
-  crypto_enc (nroot.@"m2") msg2_pred -∗
-  crypto_enc (nroot.@"m3") msg3_pred -∗
   pterm (TKey Enc kB) -∗
-  crypto_meta_token nB (↑cryptoN.@"nsl".@nB) -∗
+  crypto_meta_token nB (↑N) -∗
   sterm nB -∗
-  (∀ kA nA, |==> □ (pterm nB ↔ ▷ (pterm (TKey Dec kA) ∨ pterm (TKey Dec kB))) ∗
+  (∀ kA nA, |==> □ (pterm nB ↔ ▷ corruption kA kB) ∗
                  nsl_sess_inv Resp kA kB nA nB) -∗
   (∀ ot : option (term * term),
       (if ot is Some (pkA, nA) then
@@ -256,15 +293,14 @@ Lemma wp_responder kB E Ψ nB :
            ⌜pkA = TKey Enc kA⌝ ∧
            pterm pkA ∧
            sterm nA ∧
-           □ (pterm nA ↔ pterm nB) ∧
-           ((pterm (TKey Dec kA) ∨ pterm (TKey Dec kB)) ∨
-             nsl_sess_inv Init kA kB nA nB)
+           □ (pterm nA ↔ ▷ corruption kA kB) ∧
+           (corruption kA kB ∨ nsl_sess_inv Init kA kB nA nB)
        else True) -∗
        Ψ (repr ot)) -∗
-  WP responder (TKey Dec kB) (TKey Enc kB) nB @ E {{ Ψ }}.
+  WP nsl_resp (TKey Dec kB) (TKey Enc kB) nB @ E {{ Ψ }}.
 Proof.
-iIntros (?) "#ctx #? #? #? #e_kB unreg #s_nB set_nB Hpost".
-rewrite /responder; wp_pures.
+iIntros (?) "#ctx #e_kB unreg #s_nB set_nB Hpost".
+rewrite /nsl_resp; wp_pures.
 wp_bind (recv _); iApply wp_recv; iIntros (m1) "#Hm1".
 wp_tdec m1; last protocol_failure.
 wp_list_of_term m1; last protocol_failure.
@@ -282,36 +318,32 @@ wp_list (_ :: _ :: _ :: []); wp_term_of_list.
 iMod ("set_nB" $! kA nA) as "[#p_nB inv]".
 wp_tenc; wp_pures.
 iDestruct "Hm1" as "(e_kA & s_nA & Hm1)".
-iAssert (□ (▷ (pterm (TKey Dec kA) ∨ pterm (TKey Dec kB)) → pterm nA))%I as "#p_nA".
+iAssert (□ (▷ corruption kA kB → pterm nA))%I as "#p_nA".
   iDestruct "Hm1" as "[?|#e]"; eauto.
   by iIntros "!> ?"; iApply "e"; eauto.
 iMod (session_begin with "[] inv [unreg]") as "[#sessB close]" => //.
+  by iApply nsl_ctx_session_ctx.
 iPoseProof (pterm_msg2I with "[//] [//] e_kB s_nA [] s_nB [] sessB") as "Hm2".
-- by iIntros "!> ?"; iApply "p_nA"; eauto.
+- by iIntros "!> ?"; iApply "p_nA"; rewrite /corruption; eauto.
 - by eauto.
 wp_bind (send _); iApply wp_send => //.
 wp_pures; wp_bind (recv _); iApply wp_recv; iIntros (m3) "#Hm3".
 wp_tdec m3; last protocol_failure.
 wp_eq_term e; last protocol_failure; subst m3.
-iPoseProof (pterm_TEncE with "Hm3 [//]") as "[[_ pub]|sec]".
+iPoseProof (pterm_msg3E with "[] sessB p_nB []") as "[pub|sec]" => //.
   iSpecialize ("p_nB" with "pub").
   wp_pures. iApply ("Hpost" $! (Some (TKey Enc kA, nA))).
   iExists kA; do 4!iSplit => //.
     iModIntro; iSplit; iIntros "#?" => //.
     iDestruct "Hm1" as "[?|#Hm1]"; eauto.
-    iApply "Hm1". by iApply "p_nB".
-  iLeft. by iApply "p_nB".
-iDestruct "sec" as "(#HnB & _ & _)".
+    by iApply "Hm1".
+  by iLeft.
+iDestruct "sec" as "{p_nA} (sessA & p_nA)".
 wp_if.
-iDestruct ("HnB" with "sessB") as "{p_nA} [#sessA p_nA]".
 iMod ("close" with "sessA") as "inv".
 wp_pures.
 iApply ("Hpost" $! (Some (TKey Enc kA, nA))).
-iExists kA; do 4!iSplit => //.
-  iModIntro; iSplit; iIntros "#?" => //.
-  + iApply "p_nB". by iApply "p_nA".
-  + iApply "p_nA". by iApply "p_nB".
-by eauto.
+iExists kA; do 4!iSplit => //; by eauto.
 Qed.
 
 End NSL.
